<?xml version="1.0" encoding = "UTF-8"?>
<rdf:RDF
    xmlns="http://www.w3.org/2004/02/skos/core#"
    xmlns:rdf="http://www.w3.org/1999/02/22-rdf-syntax-ns#"
    xmlns:rdfs="http://www.w3.org/2000/01/rdf-schema#"
    xmlns:skos="http://www.w3.org/2004/02/skos/core#"
    xmlns:dc="http://purl.org/dc/elements/1.1/"
    xmlns:reg="http://metadataregistry.org/uri/schema/registry/">

<!-- Scheme: MARC21-007: Specific material designation of map -->
    <skos:ConceptScheme rdf:about="http://marc21rdf.info/terms/mapsmd#">
        <dc:title>MARC21-007: Specific material designation of map</dc:title>
    </skos:ConceptScheme>

<!-- Concept: atlas  -->
		<skos:Concept rdf:about="http://marc21rdf.info/terms/mapsmd#d" xml:lang="en">
				<skos:inScheme rdf:resource="http://marc21rdf.info/terms/mapsmd#"/>
				<reg:status rdf:resource="http://metadataregistry.org/uri/RegStatus/1001"/>
				<reg:identifier rdf:resource="4428"/>
				<skos:prefLabel xml:lang="en">atlas</skos:prefLabel>
				<skos:definition xml:lang="en">Atlases generally contain maps, related text, and other cartographic information.</skos:definition>
				<skos:notation xml:lang="en">d</skos:notation>
		</skos:Concept>
<!-- Concept: diagram  -->
		<skos:Concept rdf:about="http://marc21rdf.info/terms/mapsmd#g" xml:lang="en">
				<skos:inScheme rdf:resource="http://marc21rdf.info/terms/mapsmd#"/>
				<reg:status rdf:resource="http://metadataregistry.org/uri/RegStatus/1001"/>
				<reg:identifier rdf:resource="4429"/>
				<skos:prefLabel xml:lang="en">diagram</skos:prefLabel>
				<skos:definition xml:lang="en">Map characterized by simplified, or schematic, representation. Diagrams are graphic representations of numerical data, or of the course or results of an action or process.</skos:definition>
				<skos:notation xml:lang="en">g</skos:notation>
		</skos:Concept>
<!-- Concept: map  -->
		<skos:Concept rdf:about="http://marc21rdf.info/terms/mapsmd#j" xml:lang="en">
				<skos:inScheme rdf:resource="http://marc21rdf.info/terms/mapsmd#"/>
				<reg:status rdf:resource="http://metadataregistry.org/uri/RegStatus/1001"/>
				<reg:identifier rdf:resource="4430"/>
				<skos:prefLabel xml:lang="en">map</skos:prefLabel>
				<skos:definition xml:lang="en">Two-dimensional map. Defined as a representation normally to scale and on a flat medium, of a selection of material or abstract features on, or in relation to, the surface of the earth or of another celestial body.</skos:definition>
				<skos:notation xml:lang="en">j</skos:notation>
		</skos:Concept>
<!-- Concept: model  -->
		<skos:Concept rdf:about="http://marc21rdf.info/terms/mapsmd#q" xml:lang="en">
				<skos:inScheme rdf:resource="http://marc21rdf.info/terms/mapsmd#"/>
				<reg:status rdf:resource="http://metadataregistry.org/uri/RegStatus/1001"/>
				<reg:identifier rdf:resource="4432"/>
				<skos:prefLabel xml:lang="en">model</skos:prefLabel>
				<skos:definition xml:lang="en">Three-dimensional representation of a real object. Object may be the exact size of the original or to scale.</skos:definition>
				<skos:notation xml:lang="en">q</skos:notation>
		</skos:Concept>
<!-- Concept: other  -->
		<skos:Concept rdf:about="http://marc21rdf.info/terms/mapsmd#z" xml:lang="en">
				<skos:inScheme rdf:resource="http://marc21rdf.info/terms/mapsmd#"/>
				<reg:status rdf:resource="http://metadataregistry.org/uri/RegStatus/1001"/>
				<reg:identifier rdf:resource="4437"/>
				<skos:prefLabel xml:lang="en">other</skos:prefLabel>
				<skos:definition xml:lang="en">Specific material designation other than atlas, diagram, map, profile, model, remote-sensing image, section, view.</skos:definition>
				<skos:notation xml:lang="en">z</skos:notation>
		</skos:Concept>
<!-- Concept: profile  -->
		<skos:Concept rdf:about="http://marc21rdf.info/terms/mapsmd#k" xml:lang="en">
				<skos:inScheme rdf:resource="http://marc21rdf.info/terms/mapsmd#"/>
				<reg:status rdf:resource="http://metadataregistry.org/uri/RegStatus/1001"/>
				<reg:identifier rdf:resource="4431"/>
				<skos:prefLabel xml:lang="en">profile</skos:prefLabel>
				<skos:definition xml:lang="en">Scale representation of the intersection of a vertical surface (which may or may not be a plane) with the surface of the ground or with that of a conceptual three-dimensional model of phenomena having continuous distribution (e.g., rainfall).</skos:definition>
				<skos:notation xml:lang="en">k</skos:notation>
		</skos:Concept>
<!-- Concept: remote-sensing image  -->
		<skos:Concept rdf:about="http://marc21rdf.info/terms/mapsmd#r" xml:lang="en">
				<skos:inScheme rdf:resource="http://marc21rdf.info/terms/mapsmd#"/>
				<reg:status rdf:resource="http://metadataregistry.org/uri/RegStatus/1001"/>
				<reg:identifier rdf:resource="4433"/>
				<skos:prefLabel xml:lang="en">remote-sensing image</skos:prefLabel>
				<skos:definition xml:lang="en">Image produced by a recording device that is not in physical or intimate contact with the object under study.</skos:definition>
				<skos:notation xml:lang="en">r</skos:notation>
		</skos:Concept>
<!-- Concept: section  -->
		<skos:Concept rdf:about="http://marc21rdf.info/terms/mapsmd#s" xml:lang="en">
				<skos:inScheme rdf:resource="http://marc21rdf.info/terms/mapsmd#"/>
				<reg:status rdf:resource="http://metadataregistry.org/uri/RegStatus/1001"/>
				<reg:identifier rdf:resource="4434"/>
				<skos:prefLabel xml:lang="en">section</skos:prefLabel>
				<skos:definition xml:lang="en">Scaled representation of a vertical surface (commonly a plane) displaying both the the intersection profile or some conceptual model, and the underlying structures, e.g., geological section.</skos:definition>
				<skos:notation xml:lang="en">s</skos:notation>
		</skos:Concept>
<!-- Concept: unspecified  -->
		<skos:Concept rdf:about="http://marc21rdf.info/terms/mapsmd#u" xml:lang="en">
				<skos:inScheme rdf:resource="http://marc21rdf.info/terms/mapsmd#"/>
				<reg:status rdf:resource="http://metadataregistry.org/uri/RegStatus/1001"/>
				<reg:identifier rdf:resource="4435"/>
				<skos:prefLabel xml:lang="en">unspecified</skos:prefLabel>
				<skos:definition xml:lang="en">Unspecified.</skos:definition>
				<skos:notation xml:lang="en">u</skos:notation>
		</skos:Concept>
<!-- Concept: view  -->
		<skos:Concept rdf:about="http://marc21rdf.info/terms/mapsmd#y" xml:lang="en">
				<skos:inScheme rdf:resource="http://marc21rdf.info/terms/mapsmd#"/>
				<reg:status rdf:resource="http://metadataregistry.org/uri/RegStatus/1001"/>
				<reg:identifier rdf:resource="4436"/>
				<skos:prefLabel xml:lang="en">view</skos:prefLabel>
				<skos:definition xml:lang="en">Perspective representation of the landscape shown as if it were projected onto an oblique plane.</skos:definition>
				<skos:notation xml:lang="en">y</skos:notation>
		</skos:Concept>

<!-- Status properties used in this document  -->
    <skos:Concept rdf:about="http://metadataregistry.org/uri/RegStatus/1001">
        <skos:prefLabel xml:lang="en">Published</skos:prefLabel>
    </skos:Concept>

</rdf:RDF>