<?xml version="1.0" encoding = "UTF-8"?>
<rdf:RDF
    xmlns="http://www.w3.org/2004/02/skos/core#"
    xmlns:rdf="http://www.w3.org/1999/02/22-rdf-syntax-ns#"
    xmlns:rdfs="http://www.w3.org/2000/01/rdf-schema#"
    xmlns:skos="http://www.w3.org/2004/02/skos/core#"
    xmlns:dc="http://purl.org/dc/elements/1.1/"
    xmlns:reg="http://metadataregistry.org/uri/schema/registry/">

<!-- Scheme: MARC21-007: Generation of microform -->
    <skos:ConceptScheme rdf:about="http://marc21rdf.info/terms/microformgen#">
        <dc:title>MARC21-007: Generation of microform</dc:title>
    </skos:ConceptScheme>

<!-- Concept: first generation (master)  -->
		<skos:Concept rdf:about="http://marc21rdf.info/terms/microformgen#a" xml:lang="en">
				<skos:inScheme rdf:resource="http://marc21rdf.info/terms/microformgen#"/>
				<reg:status rdf:resource="http://metadataregistry.org/uri/RegStatus/1001"/>
				<reg:identifier rdf:resource="3872"/>
				<skos:prefLabel xml:lang="en">first generation (master)</skos:prefLabel>
				<skos:definition xml:lang="en">Camera master or COM recorder master.</skos:definition>
				<skos:notation xml:lang="en">a</skos:notation>
				<skos:scopeNote xml:lang="en">Used for all master films that are made on archival stock in accordance with archival productions standards and that are given archival storage under relevant ISO standards.</skos:scopeNote>
		</skos:Concept>
<!-- Concept: mixed generation  -->
		<skos:Concept rdf:about="http://marc21rdf.info/terms/microformgen#m" xml:lang="en">
				<skos:inScheme rdf:resource="http://marc21rdf.info/terms/microformgen#"/>
				<reg:status rdf:resource="http://metadataregistry.org/uri/RegStatus/1001"/>
				<reg:identifier rdf:resource="3875"/>
				<skos:prefLabel xml:lang="en">mixed generation</skos:prefLabel>
				<skos:definition xml:lang="en">A combination of generations of film.</skos:definition>
				<skos:notation xml:lang="en">m</skos:notation>
		</skos:Concept>
<!-- Concept: printing master  -->
		<skos:Concept rdf:about="http://marc21rdf.info/terms/microformgen#b" xml:lang="en">
				<skos:inScheme rdf:resource="http://marc21rdf.info/terms/microformgen#"/>
				<reg:status rdf:resource="http://metadataregistry.org/uri/RegStatus/1001"/>
				<reg:identifier rdf:resource="3873"/>
				<skos:prefLabel xml:lang="en">printing master</skos:prefLabel>
				<skos:definition xml:lang="en">Any generation employed mainly for the production of other microforms.</skos:definition>
				<skos:notation xml:lang="en">b</skos:notation>
				<skos:scopeNote xml:lang="en">Used for all masters that are not manufactured, produced, and stored in accordance with archival standards.</skos:scopeNote>
		</skos:Concept>
<!-- Concept: service copy  -->
		<skos:Concept rdf:about="http://marc21rdf.info/terms/microformgen#c" xml:lang="en">
				<skos:inScheme rdf:resource="http://marc21rdf.info/terms/microformgen#"/>
				<reg:status rdf:resource="http://metadataregistry.org/uri/RegStatus/1001"/>
				<reg:identifier rdf:resource="3874"/>
				<skos:prefLabel xml:lang="en">service copy</skos:prefLabel>
				<skos:definition xml:lang="en">Microform made from another microform that is intended primarily for use rather than for production of other microforms.</skos:definition>
				<skos:notation xml:lang="en">c</skos:notation>
				<skos:scopeNote xml:lang="en">Always used for microopaques.</skos:scopeNote>
		</skos:Concept>
<!-- Concept: unknown  -->
		<skos:Concept rdf:about="http://marc21rdf.info/terms/microformgen#u" xml:lang="en">
				<skos:inScheme rdf:resource="http://marc21rdf.info/terms/microformgen#"/>
				<reg:status rdf:resource="http://metadataregistry.org/uri/RegStatus/1001"/>
				<reg:identifier rdf:resource="3876"/>
				<skos:prefLabel xml:lang="en">unknown</skos:prefLabel>
				<skos:definition xml:lang="en">Generation aspect is not known.</skos:definition>
				<skos:notation xml:lang="en">u</skos:notation>
		</skos:Concept>

<!-- Status properties used in this document  -->
    <skos:Concept rdf:about="http://metadataregistry.org/uri/RegStatus/1001">
        <skos:prefLabel xml:lang="en">Published</skos:prefLabel>
    </skos:Concept>

</rdf:RDF>