<?xml version="1.0" encoding = "UTF-8"?>
<rdf:RDF
    xmlns="http://www.w3.org/2004/02/skos/core#"
    xmlns:rdf="http://www.w3.org/1999/02/22-rdf-syntax-ns#"
    xmlns:rdfs="http://www.w3.org/2000/01/rdf-schema#"
    xmlns:skos="http://www.w3.org/2004/02/skos/core#"
    xmlns:dc="http://purl.org/dc/elements/1.1/"
    xmlns:reg="http://metadataregistry.org/uri/schema/registry/">

<!-- Scheme: MARC21-007: Kind of cutting of sound recording -->
    <skos:ConceptScheme rdf:about="http://marc21rdf.info/terms/soundrecordingcut#">
        <dc:title>MARC21-007: Kind of cutting of sound recording</dc:title>
    </skos:ConceptScheme>

<!-- Concept: hill-and-dale cutting  -->
		<skos:Concept rdf:about="http://marc21rdf.info/terms/soundrecordingcut#h" xml:lang="en">
				<skos:inScheme rdf:resource="http://marc21rdf.info/terms/soundrecordingcut#"/>
				<reg:status rdf:resource="http://metadataregistry.org/uri/RegStatus/1001"/>
				<reg:identifier rdf:resource="3923"/>
				<skos:prefLabel xml:lang="en">hill-and-dale cutting</skos:prefLabel>
				<skos:definition xml:lang="en">Vertical cutting, with no lateral information intended for reproduction.</skos:definition>
				<skos:notation xml:lang="en">h</skos:notation>
				<skos:scopeNote xml:lang="en">All cylinders and some early discs have this cutting.</skos:scopeNote>
		</skos:Concept>
<!-- Concept: lateral or combined cutting  -->
		<skos:Concept rdf:about="http://marc21rdf.info/terms/soundrecordingcut#l" xml:lang="en">
				<skos:inScheme rdf:resource="http://marc21rdf.info/terms/soundrecordingcut#"/>
				<reg:status rdf:resource="http://metadataregistry.org/uri/RegStatus/1001"/>
				<reg:identifier rdf:resource="3924"/>
				<skos:prefLabel xml:lang="en">lateral or combined cutting</skos:prefLabel>
				<skos:definition xml:lang="en">Cutting containing lateral information intended for reproduction. Such discs may also have vertical components intended for reproduction.</skos:definition>
				<skos:notation xml:lang="en">l</skos:notation>
				<skos:scopeNote xml:lang="en">Most contemporary discs (i.e., all quadraphonic discs and nearly all stereophonic discs) contain both vertical and laterial information and are coded l. Monographic discs are normally lateral only.</skos:scopeNote>
		</skos:Concept>
<!-- Concept: not applicable  -->
		<skos:Concept rdf:about="http://marc21rdf.info/terms/soundrecordingcut#n" xml:lang="en">
				<skos:inScheme rdf:resource="http://marc21rdf.info/terms/soundrecordingcut#"/>
				<reg:status rdf:resource="http://metadataregistry.org/uri/RegStatus/1001"/>
				<reg:identifier rdf:resource="3925"/>
				<skos:prefLabel xml:lang="en">not applicable</skos:prefLabel>
				<skos:definition xml:lang="en">Item is not a disc or a cylinder.</skos:definition>
				<skos:notation xml:lang="en">n</skos:notation>
				<skos:scopeNote xml:lang="en">Includes compact audio discs as they are pitted rather than cut.</skos:scopeNote>
		</skos:Concept>
<!-- Concept: unknown  -->
		<skos:Concept rdf:about="http://marc21rdf.info/terms/soundrecordingcut#u" xml:lang="en">
				<skos:inScheme rdf:resource="http://marc21rdf.info/terms/soundrecordingcut#"/>
				<reg:status rdf:resource="http://metadataregistry.org/uri/RegStatus/1001"/>
				<reg:identifier rdf:resource="3926"/>
				<skos:prefLabel xml:lang="en">unknown</skos:prefLabel>
				<skos:definition xml:lang="en">Kind of cutting is not known.</skos:definition>
				<skos:notation xml:lang="en">u</skos:notation>
		</skos:Concept>

<!-- Status properties used in this document  -->
    <skos:Concept rdf:about="http://metadataregistry.org/uri/RegStatus/1001">
        <skos:prefLabel xml:lang="en">Published</skos:prefLabel>
    </skos:Concept>

</rdf:RDF>