<?xml version="1.0" encoding = "UTF-8"?>
<rdf:RDF
    xmlns="http://www.w3.org/2004/02/skos/core#"
    xmlns:rdf="http://www.w3.org/1999/02/22-rdf-syntax-ns#"
    xmlns:rdfs="http://www.w3.org/2000/01/rdf-schema#"
    xmlns:skos="http://www.w3.org/2004/02/skos/core#"
    xmlns:dc="http://purl.org/dc/elements/1.1/"
    xmlns:reg="http://metadataregistry.org/uri/schema/registry/">

<!-- Scheme: MARC21-007: Groove width/groove pitch of sound recording -->
    <skos:ConceptScheme rdf:about="http://marc21rdf.info/terms/soundrecordinggro#">
        <dc:title>MARC21-007: Groove width/groove pitch of sound recording</dc:title>
    </skos:ConceptScheme>

<!-- Concept: coarse/standard  -->
		<skos:Concept rdf:about="http://marc21rdf.info/terms/soundrecordinggro#s" xml:lang="en">
				<skos:inScheme rdf:resource="http://marc21rdf.info/terms/soundrecordinggro#"/>
				<reg:status rdf:resource="http://metadataregistry.org/uri/RegStatus/1001"/>
				<reg:identifier rdf:resource="3897"/>
				<skos:prefLabel xml:lang="en">coarse/standard</skos:prefLabel>
				<skos:definition xml:lang="en">Coarse or standard groove.</skos:definition>
				<skos:notation xml:lang="en">s</skos:notation>
				<skos:scopeNote xml:lang="en">Discs issued at 78 rpm are usually coarse. Cylinders issued at 120 rpm (which have 100 grooves per inch) are usually standard.</skos:scopeNote>
		</skos:Concept>
<!-- Concept: microgroove/fine  -->
		<skos:Concept rdf:about="http://marc21rdf.info/terms/soundrecordinggro#m" xml:lang="en">
				<skos:inScheme rdf:resource="http://marc21rdf.info/terms/soundrecordinggro#"/>
				<reg:status rdf:resource="http://metadataregistry.org/uri/RegStatus/1001"/>
				<reg:identifier rdf:resource="3895"/>
				<skos:prefLabel xml:lang="en">microgroove/fine</skos:prefLabel>
				<skos:definition xml:lang="en">Microgroove disc or a fine cylinder.</skos:definition>
				<skos:notation xml:lang="en">m</skos:notation>
				<skos:scopeNote xml:lang="en">Discs issued at 16, 33 1/3, and 45 rpm are usually issued as microgroove. Cylinders issued at 160 rpm (which have 200 grooves per inch) are usually issued as fine.</skos:scopeNote>
		</skos:Concept>
<!-- Concept: not applicable  -->
		<skos:Concept rdf:about="http://marc21rdf.info/terms/soundrecordinggro#n" xml:lang="en">
				<skos:inScheme rdf:resource="http://marc21rdf.info/terms/soundrecordinggro#"/>
				<reg:status rdf:resource="http://metadataregistry.org/uri/RegStatus/1001"/>
				<reg:identifier rdf:resource="3896"/>
				<skos:prefLabel xml:lang="en">not applicable</skos:prefLabel>
				<skos:definition xml:lang="en">Item does not contain grooves.</skos:definition>
				<skos:notation xml:lang="en">n</skos:notation>
				<skos:scopeNote xml:lang="en">Used for tapes and compact audio discs.</skos:scopeNote>
		</skos:Concept>
<!-- Concept: other  -->
		<skos:Concept rdf:about="http://marc21rdf.info/terms/soundrecordinggro#z" xml:lang="en">
				<skos:inScheme rdf:resource="http://marc21rdf.info/terms/soundrecordinggro#"/>
				<reg:status rdf:resource="http://metadataregistry.org/uri/RegStatus/1001"/>
				<reg:identifier rdf:resource="3899"/>
				<skos:prefLabel xml:lang="en">other</skos:prefLabel>
				<skos:definition xml:lang="en">Groove width/groove pitch other than microgroove/fine, coarse/standard.</skos:definition>
				<skos:notation xml:lang="en">z</skos:notation>
		</skos:Concept>
<!-- Concept: unknown  -->
		<skos:Concept rdf:about="http://marc21rdf.info/terms/soundrecordinggro#u" xml:lang="en">
				<skos:inScheme rdf:resource="http://marc21rdf.info/terms/soundrecordinggro#"/>
				<reg:status rdf:resource="http://metadataregistry.org/uri/RegStatus/1001"/>
				<reg:identifier rdf:resource="3898"/>
				<skos:prefLabel xml:lang="en">unknown</skos:prefLabel>
				<skos:definition xml:lang="en">Groove width/groove pitch is not known.</skos:definition>
				<skos:notation xml:lang="en">u</skos:notation>
		</skos:Concept>

<!-- Status properties used in this document  -->
    <skos:Concept rdf:about="http://metadataregistry.org/uri/RegStatus/1001">
        <skos:prefLabel xml:lang="en">Published</skos:prefLabel>
    </skos:Concept>

</rdf:RDF>